{
 "cells": [
  {
   "cell_type": "markdown",
   "id": "swedish-singing",
   "metadata": {},
   "source": [
    "# Study Question 4.4.1\n",
    "\n",
    "a) Using the decomposition $E[Y_{x}] = E[Y_{x}\\mid x']P(x') + E[Y_{x}\\mid x]P(x)$, we have\n",
    "\n",
    "$$\\begin{align}\n",
    "&E[Y_{X=0}] = E[Y_{X=0}|X=0]P(X=0) + E[Y_{X=0}|X=1]P(X=1)\\\\\n",
    "\\\\\n",
    "\\implies &E[Y_{X=0}|X=1] = \\frac{E[Y_{X=0}] - E[Y_{X=0}|X=0]P(X=0)}{P(X=1)}\n",
    "\\end{align}$$\n",
    "\n",
    "Since both $X$ and $Y$ are binary, we can make the following substitutions\n",
    "\n",
    "$$\\begin{align}\n",
    "&E[Y_{X=x}] = P(Y=1 \\mid \\textit{do}(X=x))\\\\\n",
    "\\\\\n",
    "&E[Y_{X=x}\\mid X=x] = P(Y=1 \\mid X=x)\n",
    "\\end{align}$$\n",
    "\n",
    "Putting it all together to calculate $\\textit{ETT}$\n",
    "\n",
    "$$\\begin{align}\n",
    "\\textit{ETT} &= E[Y_{X=1} \\mid X=1] -  E[Y_{X=0} \\mid X=1]\\\\\n",
    "\\\\\n",
    "&=P(Y=1\\mid X=1) - \\frac{P(Y=1 \\mid \\textit{do}(X=0)) - P(Y=1\\mid X=0)P(X=0)}{P(X=1)}\n",
    "\\end{align}$$\n",
    "\n",
    "The quantities above are all estimable if $P(X=x, Y=y)$ and $P(Y=y\\mid \\textit{do}(X=x))$ are known."
   ]
  },
  {
   "cell_type": "markdown",
   "id": "fifth-deposit",
   "metadata": {},
   "source": [
    "b) Let X = 0 and X = 1 be no drug and drug respectively, Z = 0 and Z = 1 be male and female respectively, and Y = 0 and Y = 1 be no recovery and recovery respectively. Table 1.1 gives us the following frequencies\n",
    "\n",
    "|X|Z|Y|n|\n",
    "|:-:|:-:|:-:|:-:|\n",
    "0|0|0|36\n",
    "1|0|0|6\n",
    "0|1|0|25\n",
    "1|1|0|71\n",
    "0|0|1|234\n",
    "1|0|1|81\n",
    "0|1|1|55\n",
    "1|1|1|192\n",
    "\n",
    "From the table\n",
    "\n",
    "$$\\begin{align}\n",
    "&P(Y=1\\mid X=0,Z=0) = \\frac{234}{270}\\\\\n",
    "&P(Y=1\\mid X=0,Z=1) = \\frac{55}{80}\\\\\n",
    "&P(Y=1\\mid X=1) = \\frac{273}{350}\\\\\n",
    "&P(Y=1\\mid X=0) = \\frac{289}{350}\\\\\n",
    "&P(X=0) = \\frac{350}{700}\\\\\n",
    "&P(X=1) = \\frac{350}{700}\\\\\n",
    "&P(Z=0) = \\frac{357}{700}\\\\\n",
    "&P(Z=1) = \\frac{343}{700}\n",
    "\\end{align}$$\n",
    "\n",
    "We need to estimate $P(Y=1\\mid \\textit{do}(X=0))$, which we can get using the adjustment formula with $Z$\n",
    "\n",
    "$$\\begin{align}\n",
    "P(Y=1\\mid \\textit{do}(X=0)) &= \\sum_{z} P(Y=1\\mid X=0,Z=z)P(Z=z)\\\\\n",
    "&= P(Y=1\\mid X=0,Z=0)P(Z=0) + P(Y=1\\mid X=0,Z=1)P(Z=1)\\\\\n",
    "&= \\frac{234}{270} \\cdot \\frac{357}{700} + \\frac{55}{80} \\cdot \\frac{343}{700}\\\\\n",
    "&= \\frac{6231}{8000}\n",
    "\\end{align}$$\n",
    "\n",
    "Using the formula from part a) we have\n",
    "\n",
    "$$\\begin{align}\n",
    "\\textit{ETT} &= \\frac{273}{350} - \\frac{\\frac{6231}{8000} - \\frac{289}{350}\\cdot\\frac{350}{700}}{\\frac{350}{700}}\\\\\n",
    "&=\\frac{1343}{28000}\n",
    "\\end{align}$$"
   ]
  },
  {
   "cell_type": "markdown",
   "id": "static-massage",
   "metadata": {},
   "source": [
    "c) By Theorem 4.3.2, we have\n",
    "$$\\textit{ETT} = E[Y_{1} - Y_{0}\\mid X=1] = E[Y\\mid\\textit{do}(x+1)] - E[Y\\mid\\textit{do}(x)]$$\n",
    "\n",
    "We calculated $P(Y=1\\mid \\textit{do}(X=0))$ in part b, so we just need $P(Y=1\\mid \\textit{do}(X=1))$\n",
    "\n",
    "$$\\begin{align}\n",
    "P(Y=1\\mid \\textit{do}(X=1)) &= \\sum_{z} P(Y=1\\mid X=1,Z=z)P(Z=z)\\\\\n",
    "&= P(Y=1\\mid X=1,Z=0)P(Z=0) + P(Y=1\\mid X=1,Z=1)P(Z=1)\\\\\n",
    "&= \\frac{81}{87} \\cdot \\frac{357}{700} + \\frac{192}{263} \\cdot \\frac{343}{700}\\\\\n",
    "&= \\frac{634983}{762700}\n",
    "\\end{align}$$\n",
    "\n",
    "Putting everything together\n",
    "\n",
    "$$\\begin{align}\n",
    "\\textit{ETT} &= \\frac{634983}{762700} - \\frac{6231}{8000}\\\\\n",
    "&= \\frac{3274803}{61016000}\n",
    "\\end{align}$$\n",
    "\n",
    "Which is an anticlimax because it's not the same as the result we obtained in part b\n",
    "\n",
    "Using the other expression given for $\\textit{ETT}$ we can verify our answer in b\n",
    "\n",
    "$$\\begin{align}\n",
    "\\textit{ETT} &= E[Y\\mid X=1] - \\sum_{z} E[Y\\mid X=0,Z=z]P(Z=z\\mid X=1)\\\\\n",
    "&= P(Y=1\\mid X=1) - \\sum_{z} P[Y=1\\mid X=0,Z=z]P(Z=z\\mid X=1)\\\\\n",
    "&= P(Y=1\\mid X=1) - (P(Y=1\\mid X=0,Z=0)P(Z=0\\mid X=1) + P(Y=1\\mid X=0,Z=1)P(Z=1\\mid X=1))\\\\\n",
    "\\end{align}$$ \n",
    "\n",
    "From the table in b)\n",
    "\n",
    "$$\\begin{align}\n",
    "&P(Z=0\\mid X=1) = \\frac{87}{350}\\\\\n",
    "&P(Z=1\\mid X=1) = \\frac{263}{350}\n",
    "\\end{align}$$\n",
    "\n",
    "Putting it all together\n",
    "\n",
    "$$\\begin{align}\n",
    "\\textit{ETT} &= \\frac{273}{350} - \\frac{234}{270}\\cdot\\frac{87}{350} - \\frac{55}{80}\\cdot\\frac{263}{350}\\\\\n",
    "&=\\frac{1343}{28000}\n",
    "\\end{align}$$ \n",
    "\n",
    "So looks like our answer to b) was correct. But we can't seem to get there with Theorem 4.3.2, so I'm officially stuck."
   ]
  },
  {
   "cell_type": "code",
   "execution_count": null,
   "id": "advisory-curtis",
   "metadata": {},
   "outputs": [],
   "source": []
  }
 ],
 "metadata": {
  "kernelspec": {
   "display_name": "Python 3",
   "language": "python",
   "name": "python3"
  },
  "language_info": {
   "codemirror_mode": {
    "name": "ipython",
    "version": 3
   },
   "file_extension": ".py",
   "mimetype": "text/x-python",
   "name": "python",
   "nbconvert_exporter": "python",
   "pygments_lexer": "ipython3",
   "version": "3.8.5"
  }
 },
 "nbformat": 4,
 "nbformat_minor": 5
}
